@prefix : <https://w3id.org/abdn/foodsafety/fs-prov#> .
@prefix owl: <http://www.w3.org/2002/07/owl#> .
@prefix rdf: <http://www.w3.org/1999/02/22-rdf-syntax-ns#> .
@prefix xml: <http://www.w3.org/XML/1998/namespace> .
@prefix xsd: <http://www.w3.org/2001/XMLSchema#> .
@prefix rdfs: <http://www.w3.org/2000/01/rdf-schema#> .
@base <https://w3id.org/abdn/foodsafety/fs-prov> .

<https://w3id.org/abdn/foodsafety/fs-prov> rdf:type owl:Ontology ;
                                            <http://purl.org/dc/terms/created> "2016-02-01T21:32:52+00:00"^^xsd:dateTime ;
                                            <http://purl.org/dc/terms/creator> "Milan Markovic" ,
                                                                               "Peter Edwards" ;
                                            <http://purl.org/dc/terms/description> """ 
        An ontology for describing provenance of HACCP-based workflows.
        """ ;
                                            <http://purl.org/dc/terms/rights> "Copyright © 2016 University of Aberdeen" ;
                                            <http://purl.org/dc/terms/title> "FS-PROV: An ontology for describing provenance of HACCP-based workflows" ;
                                            <http://web.resource.org/cc/license> <http://creativecommons.org/licenses/by-sa/3.0/> ;
                                            rdfs:isDefinedBy "" ;
                                            rdfs:label """ 
        FS-PROV Ontology.
        """ ;
                                            owl:versionInfo "1.0.0" .

#################################################################
#    Annotation properties
#################################################################

###  http://purl.org/dc/terms/created
<http://purl.org/dc/terms/created> rdf:type owl:AnnotationProperty .


###  http://purl.org/dc/terms/creator
<http://purl.org/dc/terms/creator> rdf:type owl:AnnotationProperty .


###  http://purl.org/dc/terms/description
<http://purl.org/dc/terms/description> rdf:type owl:AnnotationProperty .


###  http://purl.org/dc/terms/rights
<http://purl.org/dc/terms/rights> rdf:type owl:AnnotationProperty .


###  http://purl.org/dc/terms/title
<http://purl.org/dc/terms/title> rdf:type owl:AnnotationProperty .


###  http://web.resource.org/cc/license
<http://web.resource.org/cc/license> rdf:type owl:AnnotationProperty .


#################################################################
#    Object Properties
#################################################################

###  https://w3id.org/abdn/foodsafety/fs-prov#entity
:entity rdf:type owl:ObjectProperty ;
        rdfs:domain owl:Thing ;
        rdfs:range :WorkflowEntity ;
        rdfs:comment """ 
        A relation that links the instantiation of some fs-prov:Resource to an sc-prov:EvaluationContext. 
        The fs-prov:Resource should be restricted by an fs-prov:Constraint which is also linked to the same sc-prov:EvaluationContext
        """ .


###  https://w3id.org/abdn/foodsafety/fs-prov#hasConstraintParameter
:hasConstraintParameter rdf:type owl:ObjectProperty ;
                        rdfs:domain :Constraint ;
                        rdfs:range :Parameter ;
                        rdfs:comment """ 
        An fs-prov:hasConstraintParameter links instantiations of  fs-prov: Parameter as a source of parameter values  for an fs-prov:Constraint.
        """ .


###  https://w3id.org/abdn/foodsafety/fs-prov#hasGoal
:hasGoal rdf:type owl:ObjectProperty ;
         rdfs:domain :Plan ;
         rdfs:range :Resource ;
         rdfs:comment """ 
         A relation that links an instance of a plan to the final expected product denoted as an fs-prov:Resource.
         """ .


###  https://w3id.org/abdn/foodsafety/fs-prov#inContextOf
:inContextOf rdf:type owl:ObjectProperty ;
             rdfs:domain :Parameter ;
             rdfs:range :Resource ;
             rdfs:comment """ 
        A property that defines which fs-prov:Resource is associated with a property described as an fs-prov:Parameter.
        """ .


###  https://w3id.org/abdn/foodsafety/fs-prov#instantiatedByActivity
:instantiatedByActivity rdf:type owl:ObjectProperty ;
                        rdfs:domain :Step ;
                        rdfs:range :WorkflowActivity ;
                        rdfs:comment """ 
        A property that links an fs-prov:Step to its instantiation in  a workflow execution described by a prov:Activity. 
        """ .


###  https://w3id.org/abdn/foodsafety/fs-prov#instantiatedByEntity
:instantiatedByEntity rdf:type owl:ObjectProperty ;
                      rdfs:domain :Resource ;
                      rdfs:range :WorkflowEntity ;
                      rdfs:comment """ 
        A property that links an fs-prov:Resource to its instantiation in  a workflow execution described by a prov:Entity. 
        """ .


###  https://w3id.org/abdn/foodsafety/fs-prov#isOptionalResourceFor
:isOptionalResourceFor rdf:type owl:ObjectProperty ;
                       rdfs:domain :Resource ;
                       rdfs:range :Step ;
                       rdfs:comment """ 
         A property that links an fs-prov:Step to an fs-prov: Resource which could  be used by the instantiation of this step. 
        """ .


###  https://w3id.org/abdn/foodsafety/fs-prov#isRequiredResourceFor
:isRequiredResourceFor rdf:type owl:ObjectProperty ;
                       rdfs:domain :Resource ;
                       rdfs:range :Step ;
                       rdfs:comment """ 
        A property that links an fs-prov:Step to an fs-prov: Resource which has to be used by the instantiation of this step. 
        """ .


###  https://w3id.org/abdn/foodsafety/fs-prov#isResultOf
:isResultOf rdf:type owl:ObjectProperty ;
            rdfs:domain :Resource ;
            rdfs:range :Step ;
            rdfs:comment """ 
        A property that links an fs-prov:Step to its expected product described as fs-prov: Resource. 
        """ .


###  https://w3id.org/abdn/foodsafety/fs-prov#restrics
:restrics rdf:type owl:ObjectProperty ;
          rdfs:domain :Constraint ;
          rdfs:range :Resource ;
          rdfs:comment """ 
        A property that associates restrictions identified by an fs-prov:Constraint with a specific fs-prov:Resource. 
        """ .


#################################################################
#    Classes
#################################################################

###  https://w3id.org/abdn/foodsafety/fs-prov#Constraint
:Constraint rdf:type owl:Class ;
            rdfs:comment """ 
        An fs-prov: Constraint identifies a logical statement that describes some restrictions on fs-prov:Resource in the context of an fs-prov:Step. 
        """ .


###  https://w3id.org/abdn/foodsafety/fs-prov#HaccpConstraint
:HaccpConstraint rdf:type owl:Class ;
                 rdfs:subClassOf :Constraint ;
                 rdfs:comment """ 
                An fs-prov: HACCPConstraint identifies a logical statement that describes some restrictions on an 
                fs-prov:Resource in the context of an fs-prov:HACCPStep. fs-prov: HACCPConstraint is typically defined 
                in the context of maximum or minimum threshold values of some properties relating to an fs-prov:Resource
                """ .


###  https://w3id.org/abdn/foodsafety/fs-prov#HaccpStep
:HaccpStep rdf:type owl:Class ;
           rdfs:subClassOf :Step ;
           rdfs:comment """ 
           An fs-prov: HACCPStep denotes parts of a workflow plan which represent expected HACCP-regulated activities 
           that transform fs-prov: PhysicalObject(s).
           """ .


###  https://w3id.org/abdn/foodsafety/fs-prov#Parameter
:Parameter rdf:type owl:Class ;
           rdfs:subClassOf :Resource ;
           rdfs:comment """ 
           An fs-prov: Parameter denotes parts of a workflow plan, which can be used by an fs-prov:Constraint 
           to determine variables of a restriction defined by fs-prov:Constraint. 
           """ .


###  https://w3id.org/abdn/foodsafety/fs-prov#PhysicalObject
:PhysicalObject rdf:type owl:Class ;
                rdfs:subClassOf :Resource ;
                rdfs:comment """ 
                An fs-prov: PhysicalObject represents a certain type of non-virtual entity that can be used or produced by an fs-prov:Step.
                """ .


###  https://w3id.org/abdn/foodsafety/fs-prov#Plan
:Plan rdf:type owl:Class ;
      rdfs:comment """ 
An fs-prov:Plan is a specific type of p-plan:Plan. It is composed of fs-prov:Step(s), fs-prov:Resource(s) and fs-prov:Constraint(s). 
Individual concept mentions are expected to represent a specific part of a single unique plan.  
Hence, URI’s of these concepts are not to be reused in other plans or even within the same plan. 
""" .


###  https://w3id.org/abdn/foodsafety/fs-prov#Resource
:Resource rdf:type owl:Class ;
          rdfs:comment """ 
An fs-prov: Resource denotes parts of a workflow plan, which can be used by an 
fs-prov:Step and fs-prov:Constraint or produced by an fs-prov:Step.  
""" .


###  https://w3id.org/abdn/foodsafety/fs-prov#Step
:Step rdf:type owl:Class ;
      rdfs:comment """ 
An fs-prov: Step denotes parts of a workflow plan which represent expected activities that transform fs-prov: Resource(s).  
""" .


###  https://w3id.org/abdn/foodsafety/fs-prov#WorkflowActivity
:WorkflowActivity rdf:type owl:Class ;
                  rdfs:comment """ 
An fs-prov: WorkflowActivity is a subclass of prov:Activity and represents an instantiation of fs-prov:Step during a workflow execution.   
""" .


###  https://w3id.org/abdn/foodsafety/fs-prov#WorkflowEntity
:WorkflowEntity rdf:type owl:Class ;
                rdfs:comment """ 
An fs-prov: WorkflowEntity is a subclass of prov:Entity and represents an instantiation of fs-prov:Resorce during a workflow execution.  
""" .


###  Generated by the OWL API (version 5.1.9) https://github.com/owlcs/owlapi/